\section{Derivatives of Inverse Functions}

In this section we will figure out how to differentiate the inverse of a function. To do so, we recall that if $f$ and $g$ are inverses, then $f(g(x))=x$ for all $x$ in the domain of $f$. Differentiating and simplifying yields:
\begin{equation*}
\begin{split}
f(g(x))&=x\\
f'(g(x))g'(x)&=1\\
g'(x)&=\frac 1{f'(g(x))} \quad\text{assuming $f'(x)$ is nonzero}\\
\end{split}
\end{equation*}
So we have the following theorem.

{\color{blue} \bfseries Begin with Theorem 22 here, continue through Theorem 23 with changes as noted.}