\exercisesetinstructions{, compute the derivative of the given function in two ways:
\begin{enumerate}
\item By simplifying first, then taking the derivative, and
\item by using the Chain Rule first then simplifying.
\end{enumerate}
Verify that the two answers are the same.}

\exercise{$f(x) =\sin (\sin^{-1}x)$}{\mbox{}\\[-2\baselineskip]\parbox[t]{\linewidth}{\begin{enumext}
\item	$f(x) = x$, so $\fp(x) = 1$
\item	$\fp(x) = \cos(\sin^{-1}x)\frac{1}{\sqrt{1-x^2}} = 1$.
\end{enumext}}}

\exercise{$f(x) =\tan^{-1}(\tan x)$}{\mbox{}\\[-2\baselineskip]\parbox[t]{\linewidth}{\begin{enumext}
\item	$f(x) = x$, so $\fp(x) = 1$
\item	$\fp(x) = \frac{1}{1+\tan^2x}\sec^2 x = 1$
\end{enumext}}}

\exercise{$f(x) =\sin(\cos^{-1} x)$}{\mbox{}\\[-2\baselineskip]\parbox[t]{\linewidth}{\begin{enumext}
\item	$f(x) = \sqrt{1-x^2}$, so $\fp(x) = \frac{-x}{\sqrt{1-x^2}}$
\item	$\fp(x) = \cos (\cos^{-1}x)(\frac{1}{\sqrt{1-x^2}}) =\frac{-x}{\sqrt{1-x^2}}$
\end{enumext}}}

\exercise{$f(x) =\sin(\tan^{-1} x)$}{\mbox{}\\[-2\baselineskip]\parbox[t]{\linewidth}{\begin{enumext}
\item	$f(x)=\frac x{\sqrt{x^2+1}}$, so $\fp(x)=\frac1{(x^2+1)^{3/2}}$
\item	$\fp(x)=\cos(\tan^{-1}x)(\frac1{x^2+1})=\frac1{\sqrt{x^2+1}}\cdot\frac1{x^2+1}$
\end{enumext}}}

\exercisesetend
