\exercisesetinstructions{, compute the derivative of the given function.}

\exercise{$f(x) = x\sin x$}{$\fp(x) = \sin x + x\cos x$}

\exercise{$\ds f(t) = \frac{1}{t^2}(\csc t-4)$}{$\fp(t) = \frac{-2}{t^3}(\csc t-4) + \frac{1}{t^2}(-\csc t\cot t)$}

\exercise{$H(y)= (y^5 -2y^3)(7y^2 + y - 8) $}{$H'(y)= (y^5 -2y^3)(14y + 1) + (5y^4 -6y^2)(7y^2 + y - 8)$}

\exercise{$F(y)=\sqrt[3]{y^2}(y^2 + 9y)$}{$\Fp(y)=\dfrac83 y^{5/3}+15y^{2/3}=\frac{\sqrt[3]{y^2}(8y + 45)}3$}

\exercise{$\ds g(x) = \frac{x+7}{x-5}$}{$g'(x) = \frac{-12}{(x-5)^2}$}

\exercise{$y=\dfrac{\sqrt x}{x+4}$}{$y'=\dfrac{4-x}{2\sqrt x (x+4)^2}$}

\exercise{$g(x)=\dfrac{x}{\sqrt x +4}$}{$g'(x)=\dfrac{\sqrt x +8}{2(\sqrt x +4)^2}$}

\exercise{$\ds g(t) = \frac{t^5}{\cos t-2t^2}$}{$g'(t) = \frac{(\cos t-2t^2)(5t^4)-(t^5)(-\sin t-4t)}{(\cos t-2t^2)^2}$}

\exercise{$h(x) =\cot x - e^x$}{$h'(x) = -\csc^2x-e^x$}

\exercise{$h(t) =7t^2+6t-2$}{$h'(t) = 14t+6$}

\exercise{$\ds f(x)= \frac{x^4+2x^3}{x+2}$}{%\mbox{}\\[-2\baselineskip]\begin{enumerate}
%\item
$\fp(x) = \frac{(x+2)(4x^3+6x^2)-(x^4+2x^3)(1)}{(x+2)^2}$
%\item		$f(x) = x^3$ when $x\neq -2$, so $\fp(x) = 3x^2$.
%\item		They are equal.
%\end{enumerate}
}

\exercise{$f(x)=\dfrac{x^2-\sqrt x}{x^3}$}{$\fp(x)=-\dfrac1{x^2}+\dfrac5{2x^3\sqrt x}=\dfrac{-2x\sqrt x +5}{2x^3\sqrt x}$}

\exercise{$y=\left(\dfrac1{x^3}+\dfrac5{x^4}\right)(2x^3 - x^5)$}{$y'=-2x-5-\dfrac{10}{x^2}=-\dfrac{2x^3+5x^2+10}{x^2}$}

\exercise{$g(x)=\dfrac1{1+x+x^2+x^3}$}{$g'(x)=-\frac{1+2x+3x^2}{(1+x+x^2+x^3)^2}$}

\exercise{$p(x)=1+\dfrac1x+\dfrac1{x^2}+\dfrac1{x^3}$}{$p'(x)=-\dfrac1{x^2}-\dfrac2{x^3}-\dfrac3{x^4}=-\dfrac{x^2+2x+3}{x^4}$}

\exercise{$\ds f(x) = (16x^3+24x^2+3x)\frac{7x-1}{16x^3+24x^2+3x}$}{$\fp(x) = 7$}

\exercise{$ f(t) = t^5(\sec t + e^t)$}{$\fp(t) = 5t^4(\sec t+ e^t) + t^5(\sec t\tan t + e^t)$}

\exercise{$\ds f(x) = \frac{\sin x}{\cos x+3}$}{$\fp(x) = \frac{\sin ^2(x)+\cos ^2(x)+3 \cos (x)}{(\cos (x)+3)^2}$}

\exercise{$g(x) = e^2\big(\sin (\pi/4) - 1\big)$}{$g'(x) = 0$}

\exercise{$g(t) = 4t^3e^t - \sin t\cos t$}{$g'(t) = 12t^2e^t + 4t^3e^t - \cos^2t + \sin^2t$}

\exercise{$f(y)= y(2y^3-5y-1)(6y^2+7)$}{$\fp(y)=y(2y^3-5y-1)(12y)+y(6y^2-5)(6y^2+7)+1(2y^3-5y-1)(6y^2+7)=72 y^5-64 y^3-18 y^2-70 y-7$}

\exercise{$F(x)=(8x-1)(x^2+4x+7)(x^3-5)$}{$\Fp(x)=(8x-1)(x^2+4x+7)(3x^2)+(8x-1)(2x+4)(x^3-5)+(8)(x^2+4x+7)(x^3-5)$}

\exercise{$\ds h(t) = \frac{t^2\sin t+3}{t^2\cos t+2}$}{$h'(x) = \frac{(t^2\cos t+2)(2t\sin t+t^2\cos t)-(t^2\sin t+3)(2t\cos t-t^2\sin t)}{(t^2\cos t+2)^2}$}

\exercise{$f(x) = x^2e^x\tan x$}{$\fp(x) = 2xe^x\tan x = x^2e^x\tan x + x^2e^x\sec^2x$}

\exercise{$g(x) = 2x\sin x \sec x$}{$g'(x) = 2\sin x\sec x+2x\cos x \sec x + 2x\sin x\sec x\tan x = 2\tan x+2x+2x\tan^2x = 2\tan x+2x\sec^2x$}

\exercise{$f(x)=x\ln x$}{$\fp(x)=1+\ln x$}

\exercisesetend
