\exercisesetinstructions{, use the Quotient Rule to verify these derivatives.}

\exercise{$\dfrac{\dd}{\dd x}(\cot x) = -\csc^2 x$}{\mbox{}\\[-2\baselineskip]\parbox[t]{\linewidth}{\begin{align*}
\frac{\dd}{\dd x}(\cot x)
&=\frac{\dd}{\dd x}\left(\frac{\cos x}{\sin x}\right)\\
&=\frac{\sin x (-\sin x) - (\cos x)(\cos x)}{(\sin x)^2}\\
&=\frac{-[(\sin x)^2 + (\cos x)^2]}{(\sin x)^2}\\
&=\frac{-1}{(\sin x)^2} = -\csc^2 x
\end{align*}}}

% cut for parity
%\exercise{$\dfrac{\dd}{\dd x}(\sec x) = \sec x \tan x$}{\mbox{}\\[-2\baselineskip]\begin{align*}
%\frac{\dd}{\dd x}(\sec x)
%&=\frac{\dd}{\dd x}\left(\frac{1}{\cos x}\right)\\
%&=\frac{\cos x \cdot 0 - 1 \cdot (-\sin x)}{(\cos x)^2}\\
%&=\frac{\sin x}{(\cos x)^2} = \sec x \tan x
%\end{align*}}

\exercise{$\dfrac{\dd}{\dd x}(\csc x) = -\csc x \cot x$}{\mbox{}\\[-2\baselineskip]\parbox[t]{\linewidth}{\begin{align*}
\frac{\dd}{\dd x}(\csc x)
&=\frac{\dd}{\dd x}\left(\frac{1}{\sin x}\right)\\
&=\frac{\sin x \cdot 0 - 1 \cdot (\cos x)}{(\sin x)^2}\\
&=\frac{-\cos x}{(\sin x)^2} = -\csc x \cot x
\end{align*}}}

\exercisesetend
