\begin{exerciseset}{In Exercises}{:
\begin{enumerate}
\item Use the Product Rule to differentiate the function.
\item Manipulate the function algebraically and differentiate without the Product Rule.
\item Show that the answers from (a) and (b) are equivalent.
\end{enumerate}}

\exercise{$f(x) = x(x^2+3x)$}{\mbox{}\\[-2\baselineskip]\parbox[t]{\linewidth}{\begin{enumerate}
\item $\fp(x) = (x^2+3x) + x(2x+3)$
\item $\fp(x) = 3x^2 + 6x$
\item They are equal.
\end{enumerate}}}

\exercise{$g(x) = 2x^2(5x^3)$}{\mbox{}\\[-2\baselineskip]\parbox[t]{\linewidth}{\begin{enumerate}
\item $g'(x) = 4x(5x^3)+2x^2(15x^2)$
\item $g'(x) = 50x^4$
\item They are equal.
\end{enumerate}}}

\exercise{$h(s) = (2s-1)(s+4)$}{\mbox{}\\[-2\baselineskip]\parbox[t]{\linewidth}{\begin{enumerate}
\item $h'(s) = 2(s+4) + (2s-1)(1)$
\item $h'(s) = 4s + 7$
\item They are equal.
\end{enumerate}}}

\exercise{$f(x)= (x^2+5)(3-x^3)$}{\mbox{}\\[-2\baselineskip]\parbox[t]{\linewidth}{\begin{enumerate}
\item $\fp(x) = 2x(3-x^3)+(x^2+5)(-3x^2)$
\item $\fp(x) = -5x^4-15x^2+6x$
\item They are equal.
\end{enumerate}}}

\end{exerciseset}
