\exercisesetinstructions{, compute the derivative of the given function.}

\exercise{$f(x) = 7x^2-5x+7$}{$\fp(x) = 14x-5$}

\exercise{$g(x) = 14x^3+7x^2+11x-29$}{$g'(x) = 42x^2+14x+11$}

\exercise{$m(t) = 9t^5-\frac18t^3+3t-8$}{$m'(t) = 45t^4-\frac38t^2+3$}

\exercise{$f(\theta) = 9\sin \theta + 10\cos \theta$}{$\fp(\theta) = 9\cos \theta-10\sin\theta$}

\exercise{$f(r) = 6e^r$}{$\fp(r) = 6e^r$}

\exercise{$g(t) = 10t^4-\cos t +7\sin t$}{$g'(t) = 40t^3 + \sin t + 7\cos t$}

\exercise{$f(x) = 2\ln x - x$}{$\fp(x) = \frac2x-1$}

\exercise{$p(s) = \frac14s^4+\frac13s^3+\frac12s^2+s+1$}{$p'(s) = s^3+s^2+s+1$}

\exercise{$h(t) = e^t - \sin t - \cos t$}{$h'(t) = e^t - \cos t + \sin t$}

\exercise{$f(x) = \ln (5x^2)$}{$\fp(x) = \frac2x$}

\exercise{$f(t) = \ln (17)+ e^2 + \sin \pi/2$}{$\fp(t) = 0$}

\exercise{$g(t) = (1+3t)^2$}{$g'(t) = 18t+6$}

\exercise{$g(x) = (2x-5)^3$}{$g'(x) = 24x^2-120x+150$}

\exercise{$f(x) = (1-x)^3$}{$\fp(x) = -3x^2+6x-3$}

\exercise{$f(x) = (2-3x)^2$}{$\fp(x) = 18x-12$}

\exercise{$h(x) = \dfrac{x^5-2x^3+x^2}{x^2}$}{$h'(x)=3x^2 - 2$}

\exercise{$f(x) = \dfrac{x^2+1}{\sqrt x}$}{$\fp(x)=\dfrac{3}{2}\sqrt x  - \dfrac{1}{2x \sqrt x}$}

\exercise{$g(\theta) = \dfrac{1-\sin^2 \theta}{\cos \theta}$}{$g'(\theta)=-\sin \theta$}

\exercisesetend
