\exercisesetinstructions{:
\begin{enumerate}
\renewcommand{\theenumi}{(\alph{enumi})}
\item Use the Quotient Rule to differentiate the function.
\item Manipulate the function algebraically and differentiate without the Quotient Rule.
\item Show that the answers from (a) and (b) are equivalent.
\end{enumerate}}

\exercise{$\ds f(x)= \frac{x^2+3}{x}$}{\mbox{}\\[-2\baselineskip]\parbox[t]{\linewidth}{\begin{enumext}[start=1]
\item $\fp(x) = \frac{x(2x)-(x^2+3)1}{x^2}$
\item $\fp(x) = 1-\frac{3}{x^2}$
\item They are equal.
\end{enumext}}}

\exercise{$\ds g(x)= \frac{x^3-2x^2}{2x^2}$}{\mbox{}\\[-2\baselineskip]\parbox[t]{\linewidth}{\begin{enumext}[start=1]
\item $g'(x) = \frac{2x^2(3x^2-4x)-(x^3-2x^2)(4x)}{4x^4}$
\item $g'(x) = 1/2$
\item They are equal.
\end{enumext}}}

\exercise{$\ds h(s)= \frac{3}{4s^3}$}{\mbox{}\\[-2\baselineskip]\parbox[t]{\linewidth}{\begin{enumext}[start=1]
\item $h'(s) = \frac{4s^3(0) - 3(12s^2)}{16s^6}$
\item $h'(s) = -9/4s^{-4}$
\item They are equal.
\end{enumext}}}

\exercise{$\ds f(t)= \frac{t^2-1}{t+1}$}{\mbox{}\\[-2\baselineskip]\parbox[t]{\linewidth}{\begin{enumext}[start=1]
\item $\fp(t) = \frac{(t+1)(2t) - (t^2-1)(1)}{(t+1)^2}$
\item $f(t) = t-1$ when $t\neq -1$, so $\fp(t) = 1$.
\item They are equal.
\end{enumext}}}

\exercisesetend
