\exerciseset{In Exercises}{, find $\ds \frac{dy}{dx}$ using implicit differentiation.}{

\exercise{$x^4+y^2+y=7$\label{exer:02_06_ex_09}}{$\frac{dy}{dx} = \frac{-4x^3}{2y+1}$}

\exercise{$x^{2/5}+y^{2/5}=1$}{$\frac{dy}{dx}=-\frac{y^{3/5}}{x^{3/5}}$}

\exercise{$\cos x+\sin y=1$}{$\frac{dy}{dx}=\sin x\sec y$}

\exercise{$\ds\frac{x}{y}=10$\label{exer:02_06_ex_12}}{$\frac{dy}{dx}=\frac{y}{x}$}

\exercise{$\ds\frac{y}{x}=10$}{$\frac{dy}{dx}=\frac{y}{x}$}

%\exercise{$x^2e^2+2^y=5$}{$-\frac{e^x x (x+2) 2^{-y}}{\ln\abs2}$}

\exercise{$x^2e^2+e^y=5$}{$-e^x x (x+2) e^{-y}$}

\exercise{$x^2\tan y=50$}{$-\frac{2 \sin (y) \cos (y)}{x}$}

\exercise{$(3 x^2+2 y^3)^4=2$}{$-\frac{x}{y^2}$}

\exercise{$(y^2+2y-x)^2=200$}{$\frac{1}{2y+2}$}

\exercise{$\ds\frac{x^2+y}{x+y^2}=17$}{$\frac{x^2+2 x y^2-y}{2 x^2 y-x+y^2}$}

\exercise{$\ds\frac{\sin (x)+y}{\cos (y)+x}=1$}{$\frac{-\cos (x) (x+\cos (y))+\sin (x)+y}{\sin (y) (\sin (x)+y)+x+\cos (y)}$}

\exercise{$\ln (x^2+y^2) = e$}{$-\frac{x}{y}$}

\exercise{$\ln (x^2+xy+y^2) = 1$}{$-\frac{2x+y}{2y+x}$}

\exercise{$xe^x = ye^y$}{$\dfrac{e^x(x+1)}{e^y(y+1)}$}

\exercise{$y\sin(x^3) = x\sin(y^3)$}{$\dfrac{3x^2y\cos x^3 - \sin y^3}{3xy^2\sin y^3 - \sin x^3}$}

\exercise{$\sqrt{xy} = 1 + x^2y$}{$\dfrac{y-4xy\sqrt{xy}}{2x^2\sqrt{xy}-x}$}

%\printreview

\exercise{%Find $\dfrac{dy}{dx}$, where 
$x^2y-y^2x = 1$}{$\frac{dy}{dx} = \frac{y (y-2 x)}{x (x-2 y)}$}

\exercise{%Find the derivative of %equation of the line tangent to the graph of\\
$x^2+y^2+xy=7$}{$\frac{dy}{dx}=-\frac{y+2x}{2y+x}$}% { at the point $(1,2)$.}{$-\frac45$}%{$y=-\frac45(x-1)+2$}

%\exercise{Let $f(x) = x^3+x$. Evaluate $\ds \lim_{s\to 0} \frac{f(x+s)-f(x)}{s}$.}{ $3x^2+1$}

%\exercise{Approximate the value of $(3.01)^4$ using the tangent line to $f(x) = x^4$ at $x=3$.}{The tangent line to $f(x) = x^4$ at $x=3$ is $y=108(x-3)+81$; thus $(3.01)^4 \approx y(3.01) = 108(.01)+81 = 82.08$. }

% (1/2)(xy)^{-1/2}(xy'+y) = x^2 y' + 2xy
% xy'+y = 2x^{5/2}y^{1/2}y' + 4 x^{3/2}y^{3/2}
% (x-2x^{5/2}y^{1/2})y' = 4x^{3/2}y^{3/2}-y
%
% y' = (4x^{3/2}y^{3/2}-y) / (x-2x^{5/2}y^{1/2})

}
