\exerciseset{In Exercises}{:
\begin{enumerate}
\item[(a)] Use the Quotient Rule to differentiate the function.
\item[(b)] Manipulate the function algebraically and differentiate without the Quotient Rule.
\item[(c)] Show that the answers from (a) and (b) are equivalent.
\end{enumerate}
}{

\exercise{$\ds f(x)= \frac{x^2+3}{x}$
}{\begin{enumerate}
\item		$\fp(x) = \frac{x(2x)-(x^2+3)1}{x^2}$
\item		$\fp(x) = 1-\frac{3}{x^2}$
\item		They are equal.
\end{enumerate}
}

\exercise{$\ds g(x)= \frac{x^3-2x^2}{2x^2}$
}{\begin{enumerate}
\item		$g'(x) = \frac{2x^2(3x^2-4x)-(x^3-2x^2)(4x)}{4x^4}$
\item		$g'(x) = 1/2$
\item		They are equal.
\end{enumerate}
}

\exercise{$\ds h(s)= \frac{3}{4s^3}$
}{\begin{enumerate}
\item		$h'(s) = \frac{4s^3(0) - 3(12s^2)}{16s^6}$
\item		$h'(s) = -9/4s^{-4}$
\item		They are equal.
\end{enumerate}
}

\exercise{$\ds f(t)= \frac{t^2-1}{t+1}$
}{\begin{enumerate}
\item		$\fp(t) = \frac{(t+1)(2t) - (t^2-1)(1)}{(t+1)^2}$
\item		$f(t) = t-1$ when $t\neq -1$, so $\fp(t) = 1$.
\item		They are equal.
\end{enumerate}
}
}