\exerciseset{In Exercises}{, compute the derivative of the given function.}{

\exercise{$f(x) = (4x^3-x)^{10}$\label{exer:02_05_06}}{$\fp(x) = 10(4x^3-x)^9\cdot(12x^2-1) = (120x^2-10)(4x^3-x)^9$}

\exercise{$f(t) = (3t-2)^{5}$}{$\fp(t) = 15(3t-2)^4$}

\exercise{$g(\theta) = (\sin \theta+\cos \theta)^3$}{$g'(\theta) = 3(\sin \theta+\cos \theta)^2(\cos \theta-\sin\theta)$}

\exercise{$h(t) = e^{3t^2+t-1}$\label{exer:02_05_09}}{$h'(t) = (6t+1)e^{3t^2+t-1}$}

\exercise{$f(x) = \big(x+\frac{1}{x}\big)^4$}{$\fp(x) = 4\big(x+\frac1x\big)^3\big(1-\frac{1}{x^2}\big)$}

\exercise{$p(x) = \left(x^2 - \dfrac{1}{x^2}\right)^6$}{$p'(x) = 12\left(x^2 - \dfrac{1}{x^2}\right)^5 \left(x + \dfrac{1}{x^3}\right)$}

\exercise{$f(x) = \cos (3x)$}{$\fp(x) = -3\sin(3x)$}

\exercise{$g(x) = \tan (5x)$}{$g'(x) = 5\sec^2(5x)$}

\exercise{$h(t) = \sin^4(2t)$}{$h'(t) = 8\sin^3(2t)\cos(2t)$}

\exercise{$p(t) = \cos^3(t^2+3t+1)$}{$p'(t) = -3\cos^2(t^2+3t+1)\sin(t^2+3t+1)(2t+3)$}

\exercise{$g(x) = \tan^2 x - \tan (x^2)$}{$g'(x) = 2(\tan x \sec^2 x - x \sec^2 (x^2))$}

\exercise{$w(x) = \sec (e^{x^3})$}{$w'(x) = 3x^2 e^{x^3}(\sec e^{x^3})(\tan e^{x^3})$}

\exercise{$f(x) = \ln (\cos x)$}{$\fp(x) = -\tan x$}

\exercise{$f(x) = \ln (x^2)$}{$\fp(x) = 2/x$}

\exercise{$f(x) = 2\ln (x)$}{$\fp(x) = 2/x$}

%\exercise{$g(r) = 4^r$}{$g'(r) = \ln 4\cdot 4^r$}

%\exercise{$g(t) = 5^{\cos t}$}{$g'(t) = -\ln 5\cdot 5^{\cos t}\sin t$}

\exercise{$g(t) = 15^2$}{$g'(t) = 0$}

\exercise{$r(x) = \dfrac{\sqrt {4x-3}}{x^2}$}{$r'(x) = \dfrac{-6(x-1)}{x^3 \sqrt {4x-3}}$}

\exercise{$f(x) = \dfrac {(3x^2 - 5)^4}{(2x^3-1)^2}$}{$\fp(x) = \dfrac {12x(2x^3-1)(3x^2 - 5)^3(x^2+5x-2)}{(2x^3-1)^4}$}

\exercise{$h(x)=[(2x+1)^{10} + 1]^{10}$}{$h'(x)=200(2x+1)^9[(2x+1){10}+1]^9$}

\exercise{$f(t)=\left[\left(1+ \dfrac{1}{t}\right)^{-1} + 1\right]^{-1}$}{$\fp(t)=\dfrac{-t^4}{(2t+1)(t+1)}$}

\exercise{$F(x)=2x(2x+1)^2 (2x+3)^3$}{$\Fp(x)=2(2x+1)(2x+3)^2(24x^2+26x+3)$}

%\exercise{$\ds m(w) = \frac{3^w}{2^w}$}{$m'(w) = \ln (3/2) (3/2)^w$}

%\exercise{$\ds h(t) = \frac{2^t+3}{3^t+2}$}{$\fp(x) = \frac{(3^t+2)\big((\ln 2) 2^t\big)-(2^t+3)\big((\ln 3)3^t\big)}{(3^t+2)^2}$}

%\exercise{$\ds m(w) = \frac{3^w+1}{2^w}$}{$m'(w) = \frac{2^w\big(\ln 3\cdot 3^w-\ln 2\cdot (3^w+1)\big)}{2^{2w}}$}

%\exercise{$\ds f(x) = \frac{3^{x^2}+x}{2^{x^2}}$}{$\fp(x) = \frac{2^{x^2}(\ln 3\cdot 3^x{x^2}2x+1) - (3^{x^2}+x)(\ln 2\cdot 2^{x^2}2x)}{2^{2x^2}}$}

\exercise{$f(x) = x^2\sin(5x)$}{$\fp(x) = 5x^2\cos(5x) + 2x\sin(5x)$}

\exercise{$g(t)   = \cos(t^2+3t)\sin(5t-7)$}{$g'(t) = 5\cos(t^2+3t)\cos(5t-7)- (2t+3)\sin(t^2+3t)\sin(5t-7)$}

\exercise{$g(t)   = \cos(\frac1t)e^{5t^2}$}{$g'(t) = 10t\cos(\frac1t)e^{5t^2}+\frac{1}{t^2}\sin(\frac1t)e^{5t^2}$}

\exercise{$a(t) = 7t^3e^{\tan t^2}$}{$a'(t)=7t^2 e^{\tan (t^2)}(2t^2 \sec^2 (t^2) + 3)$}

\exercise{$y=\sqrt{\sin (\cos^2 x)}$}{$y'=\dfrac{-\cos x \sin x \cos (\cos^2 x)}{\sqrt{\sin (\cos^2 x)}}$}

\exercise{$k(x) = \cos(x\sin x^3)$}{$k'(x) = -\sin(x\sin x^3)(3x^3\cos x^3 + \sin x^3)$}

}
