\exerciseset{In Exercises}{, use the Quotient Rule to verify these derivatives.
}{

\exercise{$\dfrac{d}{dx}(\cot x) = -\csc^2 x$}{\begin{align*}
\frac{d}{dx}(\cot x)
&=\frac{d}{dx}\left(\frac{\cos x}{\sin x}\right)\\
&=\frac{\sin x (-\sin x) - (\cos x)(\cos x)}{(\sin x)^2}\\
&=\frac{-[(\sin x)^2 + (\cos x)^2]}{(\sin x)^2}\\
&=\frac{-1}{(\sin x)^2} = -\csc^2 x
\end{align*}}

\exercise{$\dfrac{d}{dx}(\sec x) = \sec x \tan x$}{\begin{align*}
\frac{d}{dx}(\sec x)
&=\frac{d}{dx}\left(\frac{1}{\cos x}\right)\\
&=\frac{\cos x \cdot 0 - 1 \cdot (-\sin x)}{(\cos x)^2}\\
&=\frac{\sin x}{(\cos x)^2} = \sec x \tan x
\end{align*}}

\exercise{$\dfrac{d}{dx}(\csc x) = -\csc x \cot x$}{\begin{align*}
\frac{d}{dx}(\csc x)
&=\frac{d}{dx}\left(\frac{1}{\sin x}\right)\\
&=\frac{\sin x \cdot 0 - 1 \cdot (\cos x)}{(\sin x)^2}\\
&=\frac{-\cos x}{(\sin x)^2} = -\csc x \cot x
\end{align*}}

}