\exerciseset{In Exercises}{, compute the derivative of the given relation.}{

\exercise{$f(x) = (2-3x)^2$}{$\fp(x) = 18x-12$}

\exercise{$f(x) = x^2\sin(5x)$}{$\fp(x) = 5x^2\cos(5x) + 2x\sin(5x)$}

\exercise{$f(r) = 6e^r$}{$\fp(r) = 6e^r$}

\exercise{$x^{2/5}+y^{2/5}=1$}{$\frac{dy}{dx}=-\frac{y^{3/5}}{x^{3/5}}$}

\exercise{$f(x) = (4x^3-x)^{10}$\label{exer:02_05_06}}{$\fp(x) = 10(4x^3-x)^9\cdot(12x^2-1) = (120x^2-10)(4x^3-x)^9$}

\exercise{$g(t) = (1+3t)^2$}{$g'(t) = 18t+6$}

\exercise{$f(x) = \big(x+\frac{1}{x}\big)^4$}{$\fp(x) = 4\big(x+\frac1x\big)^3\big(1-\frac{1}{x^2}\big)$}

\exercise{$g(t)   = \cos(\frac1t)e^{5t^2}$}{$g'(t) = 10t\cos(\frac1t)e^{5t^2}+\frac{1}{t^2}\sin(\frac1t)e^{5t^2}$}

\exercise{$g(t) = 15^2$}{$g'(t) = 0$}

\exercise{$\ds m(w) = \frac{3^w+1}{2^w}$}{$m'(w) = \frac{2^w\big(\ln 3\cdot 3^w-\ln 2\cdot (3^w+1)\big)}{2^{2w}}$}

\exercise{$f(x) = x\sin x$}{$\fp(x) = \sin x + x\cos x$}

\exercise{$x^2e^2+2^y=5$}{$-\frac{e^x x (x+2) 2^{-y}}{\ln\abs2}$}

\exercise{$h(x) =\cot x - e^x$}{$h'(x) = -\csc^2x-e^x$}

\exercise{$f(x) = \cos (3x)$}{$\fp(x) = -3\sin(3x)$}

\exercise{$g(r) = 4^r$}{$g'(r) = \ln 4\cdot 4^r$}

\exercise{$\ds f(x) = x^\pi+x^{1.9} + \pi^{1.9}$}{$\fp(x) = \pi x^{\pi-1}+1.9x^{0.9}$}

\exercise{$f(x) = 7x^2-5x+7$}{$\fp(x) = 14x-5$}

\exercise{$g(x) = 14x^3+7x^2+11x-29$}{$g'(x) = 42x^2+14x+11$}

\exercise{$g(x) = e^2\big(\sin (\pi/4) - 1\big)$}{$g'(x) = 0$}

\exercise{$f(\theta) = 9\sin \theta + 10\cos \theta$}{$\fp(\theta) = 9\cos \theta-10\sin\theta$}

\exercise{$g(x) = 2x\sin x \sec x$}{$g'(x) = 2\sin x\sec x+2x\cos x \sec x + 2x\sin x\sec x\tan x = 2\tan x+2x+2x\tan^2x = 2\tan x+2x\sec^2x$}

\exercise{$ f(t) = \sqrt[5]{t}(\sec t + e^t)$}{$\fp(t) = \frac15x^{-4/5}(\sec t+ e^t) + \sqrt[5]{t}(\sec t\tan t + e^t)$}

\exercise{$f(x) = 2\ln x - x$}{$\fp(x) = \frac2x-1$}

\exercise{$f(x) = \ln (5x^2)$}{$\fp(x) = \frac2x$}

\exercise{$h(x) = x^{1.5}$}{$h'(x) = 1.5x^{0.5} = 1.5\sqrt{x}$}

\exercise{$g(t) = \sqrt{t}\sin t$}{$g'(t) = \sqrt{t}\cos t + \frac{\sin t}{2\sqrt{t}}$}

\exercise{$g(x) = \tan (5x)$}{$g'(x) = 5\sec^2(5x)$}

\exercise{$f(x) = (1-x)^3$}{$\fp(x) = -3x^2+6x-3$}

\exercise{$x^2\tan y=50$}{$-\frac{2 \sin (y) \cos (y)}{x}$}

\exercise{$f(t) = (3t-2)^{5}$}{$\fp(t) = 15(3t-2)^4$}

\exercise{$g(t)   = \cos(t^2+3t)\sin(5t-7)$}{$g'(t) = 5\cos(t^2+3t)\cos(5t-7)- (2t+3)\sin(t^2+3t)\sin(5t-7)$}

\exercise{$h(t) =7t^2+6t-2$}{$h'(t) = 14t+6$}

\exercise{$\ln (x^2+xy+y^2) = 1$}{$-\frac{2x+y}{2y+x}$}

\exercise{$\ds f(x) = \frac{\sin x}{\cos x+3}$}{$\fp(x) = \frac{\sin ^2(x)+\cos ^2(x)+3 \cos (x)}{(\cos (x)+3)^2}$}

\exercise{$h(t) = e^t - \sin t - \cos t$}{$h'(t) = e^t - \cos t + \sin t$}

\exercise{$p(s) = \frac14s^4+\frac13s^3+\frac12s^2+s+1$}{$p'(s) = s^3+s^2+s+1$}

\exercise{$g(\theta) = (\sin \theta+\cos \theta)^3$}{$g'(\theta) = 3(\sin \theta+\cos \theta)^2(\cos \theta-\sin\theta)$}

\exercise{$g(t) = 5^{\cos t}$}{$g'(t) = -\ln 5\cdot 5^{\cos t}\sin t$}

\exercise{$p(t) = \cos^3(t^2+3t+1)$}{$p'(t) = -3\cos^2(t^2+3t+1)\sin(t^2+3t+1)(2t+3)$}

\exercise{$g(t) = 4t^3e^t - \sin t\cos t$}{$g'(t) = 12t^2e^t + 4t^3e^t - \cos^2t + \sin^2t$}

}
