\exerciseset{In Exercises}{, verify the given identity using Definition \ref{def:hyperbolic_functions}, as done in Example \ref{ex_hf1}.}{

\exercise{$\coth^2 x-\csch^2x=1$}{\hfill$\begin{aligned}[t]
		\coth^2x-\csch^2x &= \left(\frac{e^x+e^{-x}}{e^x-e^{-x}}\right)^2 - \left(\frac{2}{e^x-e^{-x}}\right)^2 \\
											&= \frac{(e^{2x} + 2 + e^{-2x}) - (4)}{e^{2x} - 2 + e^{-2x}}\\
											&= \frac{e^{2x} - 2 + e^{-2x}}{e^{2x} - 2 + e^{-2x}}\\
											&= 1										
\end{aligned}$\hfill\null}

\exercise{$\cosh 2x = \cosh^2x+\sinh^2x$}{\hfill$\begin{aligned}[t]
		\cosh^2x+\sinh^2x &= \left(\frac{e^x+e^{-x}}{2}\right)^2 + \left(\frac{e^x-e^{-x}}{2}\right)^2 \\
											&= \frac{e^{2x} + 2 + e^{-2x}}{4} + \frac{e^{2x} - 2 + e^{-2x}}{4}\\
											&= \frac{2e^{2x}  + 2e^{-2x}}{4}\\
											&= \frac{e^{2x} + e^{-2x}}{2} \\
											&= \cosh 2x.			
\end{aligned}$\hfill\null}

\exercise{$\ds\cosh^2x = \frac{\cosh2x+1}{2}$}{\hfill$\begin{aligned}[t]
		\cosh^2x &= \left(\frac{e^x+e^{-x}}{2}\right)^2  \\
											&= \frac{e^{2x} + 2 + e^{-2x}}{4} \\
											&= \frac12\frac{(e^{2x}  + e^{-2x})+2}{2}\\
											&= \frac12\left(\frac{e^{2x}  + e^{-2x}}{2}+1\right)\\
											&= \frac{\cosh2x+1}{2}.			
\end{aligned}$\hfill\null}

\exercise{$\ds\sinh^2x = \frac{\cosh2x-1}{2}$}{\hfill$\begin{aligned}[t]
		\sinh^2x &= \left(\frac{e^x-e^{-x}}{2}\right)^2  \\
											&= \frac{e^{2x} - 2 + e^{-2x}}{4} \\
											&= \frac12\frac{(e^{2x}  + e^{-2x})-2}{2}\\
											&= \frac12\left(\frac{e^{2x}  + e^{-2x}}{2}-1\right)\\
											&= \frac{\cosh2x-1}{2}.			
\end{aligned}$\hfill\null}

\exercise{$\ds\frac{d}{dx}\left[\sech x\right] = -\sech x\tanh x$}{\hfill$\begin{aligned}[t]
		\frac{d}{dx}\left[\sech x\right] &= \frac{d}{dx}\left[\frac{2}{e^x+e^{-x}}\right]  \\
											&= \frac{-2(e^x-e^{-x})}{(e^x+e^{-x})^2} \\
											&= -\frac{2(e^x-e^{-x})}{(e^x+e^{-x})(e^x+e^{-x})} \\
											&= -\frac{2}{e^x+e^{-x}}\cdot \frac{e^x-e^{-x}}{e^x+e^{-x}}\\
											&= -\sech x\tanh x
\end{aligned}$\hfill\null}

\exercise{$\ds\frac{d}{dx}\left[\coth x\right] = -\csch^2x$}{\hfill$\begin{aligned}[t]
		\frac{d}{dx}\left[\coth x\right] &= \frac{d}{dx}\left[\frac{e^x+e^{-x}}{e^x-e^{-x}}\right]  \\
											&= \frac{(e^x-e^{-x})(e^x-e^{-x})-(e^x+e^{-x})(e^x+e^{-x})}{(e^x-e^{-x})^2}\\
											&= \frac{e^{2x}+e^{-2x} - 2 - (e^{2x}+e^{-2x}+2)}{(e^x-e^{-x})^2}\\
											&= -\frac{4}{(e^x-e^{-x})^2}\\
											&=-\csch^2x
\end{aligned}$\hfill\null}

\exercise{$\ds \int \tanh x\ dx  = \ln (\cosh x) + C$}{$\ds	\int \tanh x\ dx = \int \frac{\sinh x}{\cosh x}\ dx$\\
Let $u = \cosh x$; $du = (\sinh x) dx$\\
\hfill$\begin{aligned}[t]
											&= \int \frac{1}{u}\ du \\
											&= \ln |u| + C \\
											&= \ln (\cosh x) + C.
\end{aligned}$\hfill\null}

\exercise{$\ds \int \coth x\ dx  = \ln |\sinh x| + C$}{\hfill$\begin{aligned}[t]
		\int \coth x\ dx &= \int \frac{\cosh x}{\sinh x}\ dx\\
											\text{Let $u = \sinh x$; $du = (\cosh x) dx$} 	\\
											&= \int \frac{1}{u}\ du \\
											&= \ln |u| + C \\
											&= \ln |\sinh x| + C.
\end{aligned}$\hfill\null}
}