\printconcepts

\exercise{We adopt the convention that $x^0=$\underlinespace, regardless of the value of $x$.}{1}

\exercise{What is the difference between the radius of convergence and the interval of convergence?}{The radius of convergence is a \textbf{value} $R$ such that a power series, centered at $x=c$, converges for all values of $x$ in $(c-R,c+R)$. The interval of convergence is an \textbf{interval} on which the power series converges; it may differ from $(c-R,c+R)$ only at the endpoints.}

\exercise{If the radius of convergence of $\ds\sum_{n=0}^\infty a_nx^n$ is 5, what is the radius of convergence of $\ds\sum_{n=1}^\infty n\cdot a_nx^{n-1}$?}{5}

\exercise{If the radius of convergence of $\ds\sum_{n=0}^\infty a_nx^n$ is 5, what is the radius of convergence of $\ds\sum_{n=0}^\infty (-1)^na_nx^n$?}{5}

\printproblems

\input{exercises/08-06-exset-01}

\input{exercises/08-06-exset-02}

\exercisesetinstructions{, write the following functions as a %power
% the last one isn't a power series because of the n/3
series and give the radius of convergence.}

\exercise{$\ds f(x)=\frac{x}{1-8x}$}{$\ds\sum_{n=0}^\infty 8^{n}x^{n+1}$, $R=1/8$}

% cut for parity
%\exercise{$\ds f(x)=\frac{x^7}{8+x^3}$}{$\ds\frac18\sum_{n=0}^\infty (-2)^{-3n}x^{3n+7}$, $R=2$}

\exercise{$\ds f(x)=\frac{6}{1+7x^4}$}{$\ds \sum_{n=0}^\infty 6(-7)^nx^{4n}$, $R=1/\sqrt[4]7$}

\exercise{$\ds f(x)=\frac{x^3}{3-x^2}$}{$\ds \sum_{n=0}^\infty \frac{x^{2n+3}}{3^{n+1}}$, $R=\sqrt3$}

\exercise{$\ds f(x)=\frac{3x^2}{5-2\sqrt[3]x}$}{$\ds \sum_{n=0}^\infty \frac{3\cdot2^n x^{n/3+2}}{5^{n+1}}$, $R=125/8$}

\exercisesetend

\input{exercises/08-06-exset-03}

\exercise{\mbox{}\\[-2\baselineskip]\parbox[t]{\linewidth}{\begin{enumext}[start=1]
\item Use differentiation to find a power series representation for $f(x)=\dfrac1{(1+x)^2}$. What is the radius of convergence?
\item Use part (a) to find a power series for $f(x)=\dfrac1{(1+x)^3}$.
\item Use part (b) to find a power series for $f(x)=\dfrac{x^2}{(1+x)^3}$.
\end{enumext}}}{\mbox{}\\[-2\baselineskip]\parbox[t]{\linewidth}{\begin{enumext}[start=1]
\item $\sum_{n=0}^\infty x^n(-1)^n(1+n)$; $R=1$
\item $\sum_{n=1}^\infty x^{n-1}(-1)^{n-1}(1+n)n/2\\
=\sum_{n=0}^\infty x^n(-1)^n(2+n)(1+n)/2$
\item $\sum_{n=1}^\infty x^{n+1}(-1)^{n-1}(1+n)n/2\\
=\sum_{n=0}^\infty x^{n+2}(-1)^n(2+n)(1+n)/2\\
=\sum_{n=2}^\infty x^n(-1)^n n(-1+n)/2$
\end{enumext}}}

%\input{exercises/08-06-exset-04} % uses series to solve DEs

\exercise{Suppose that $\ds \sum_{n=0}^\infty c_n x^n$ converges for $x=-3$ and diverges when $x=7$. What can you say about the convergence or divergence of the following series?
\begin{enumext}[start=1]
 \item  $\ds \sum_{n=0}^\infty c_n$
\item  $\ds \sum_{n=0}^\infty c_n 9^n$
\item  $\ds \sum_{n=0}^\infty c_n(-2)^n$
\item  $\ds \sum_{n=0}^\infty (-1)^n c_n 8^n$
\end{enumext}}{\begin{enumext}[start=1]
 \item  Converges
\item  Diverges
\item  Converges
\item  Diverges
\end{enumext}}

%\exercise{$\ds f(x)=\frac{1}{(1+x)^2}$}{$\ds\sum_{n=0}^\infty (n+1)(-1)^n x^n$, $R=1$}

%\exercise{$\ds f(x)=\frac{1}{(1+x)^3}$}{$\ds\frac12\sum_{n=0}^\infty (n+2)(n+1)(-1)^n x^n$, $R=1$}

\input{exercises/08-06-exset-05}
