\exercisesetinstructions{, use the Taylor series  given in \autoref{idea:common_taylor} to verify the given identity.}

\exercise{$\cos(-x) = \cos x$}{Given $\ds \cos x = \sum_{n=0}^\infty (-1)^n\frac{x^{2n}}{(2n)!}$,\\
$\ds\cos (-x) = \sum_{n=0}^\infty (-1)^n\frac{(-x)^{2n}}{(2n)!}=\sum_{n=0}^\infty (-1)^n\frac{x^{2n}}{(2n)!}=\cos x$, as all powers in the series are even.}

\exercise{$\sin(-x) = -\sin x$}{Given $\ds \sin x = \sum_{n=0}^\infty (-1)^n\frac{x^{2n+1}}{(2n+1)!}$,\\
$\ds\sin (-x) = \sum_{n=0}^\infty (-1)^n\frac{(-x)^{2n+1}}{(2n+1)!}=\sum_{n=0}^\infty (-1)^n\frac{-x^{2n+1}}{(2n+1)!}=-\sin x$, as all powers in the series are odd.}

\exercise{$\frac{\dd}{\dd x}\big(\sin x\big) = \cos x$}{Given $\ds \sin x = \sum_{n=0}^\infty (-1)^n\frac{x^{2n+1}}{(2n+1)!}$,\\
$\ds\frac{\dd}{\dd x}\big(\sin x\big)  = \frac{\dd}{\dd x}\left(\sum_{n=0}^\infty (-1)^n\frac{x^{2n+1}}{(2n+1)!}\right)
=\sum_{n=0}^\infty (-1)^n\frac{(2n+1)x^{2n}}{(2n+1)!}=\sum_{n=0}^\infty (-1)^n\frac{x^{2n}}{(2n)!}=\cos x$.
(The summation still starts at $n=0$ as there was no constant term in the expansion of $\sin x$).}

\exercise{$\frac{\dd}{\dd x}\big(\cos x\big) = -\sin x$}{Given $\ds \cos x = \sum_{n=0}^\infty (-1)^n\frac{x^{2n}}{(2n)!}$,\\
$\ds\frac{\dd}{\dd x}\big(\cos x\big)  = \frac{\dd}{\dd x}\left(\sum_{n=0}^\infty (-1)^n\frac{x^{2n}}{(2n)!}\right)
=\sum_{n=1}^\infty (-1)^n\frac{(2n)x^{2n-1}}{(2n)!}=\sum_{n=1}^\infty (-1)^n\frac{x^{2n-1}}{(2n-1)!}$. We can re-index this summation to start at $n=0$ by replacing $n$ with $n+1$ in the summation:
\[\sum_{n=1}^\infty (-1)^n\frac{x^{2n-1}}{(2n-1)!} =\sum_{n=0}^\infty (-1)^{n+1}\frac{x^{2n+1}}{(2n+1)!}.\]

Note that this series has the opposite sign of the Taylor series for $\sin x$; thus $\frac{\dd}{\dd x}(\cos x) = -\sin x$.}

\exercisesetend
