\exerciseset{In Exercises}{, show that the Taylor series for $f(x)$, as given in Key Idea \ref{idea:common_taylor}, is equal to $f(x)$ by applying Theorem \ref{thm:function_series_equality}; that is, show $\ds \lim_{n\to\infty}R_n(x) =0$.
}{

\exercise{$f(x) = e^x$
}{Given a value $x$, the magnitude of the error term $R_n(x)$ is bounded by
$$ \big|R_n(x)\big| \leq \frac{\max\left|\,f\,^{(n+1)}(z)\right|}{(n+1)!}\big|x^{(n+1)}\big|,$$
where $z$ is between $0$ and $x$. 

If $x>0$, then $z<x$ and $f\,^{(n+1)}(z) =e^z<e^x$. If $x<0$, then $x<z<0$ and $f\,^{(n+1)}(z) =e^z<1$. So given a fixed $x$ value, let $M = \max\{e^x,1\}$; $f\,^{(n)}(z)<M.$ This allows us to state

$$ \big|R_n(x)\big| \leq \frac{M}{(n+1)!}\big|x^{(n+1)}\big|.$$
For any $x$, $\ds\lim_{n\to\infty} \frac{M}{(n+1)!}\big|x^{(n+1)}\big|= 0$. Thus by the Squeeze Theorem, we conclude that $\ds \lim_{n\to\infty} R_n(x) = 0$ for all $x$, and hence
$$e^x = \sum_{n=0}^\infty \frac{x^{n}}{n!}\quad \text{for all $x$}.$$
}
\exercise{$f(x) = \sin x$
}{The following argument is essentially the same as that given for $f(x) = \cos x$ in Example \ref{ex_ts3}.

Given a value $x$, the magnitude of the error term $R_n(x)$ is bounded by
$$ \big|R_n(x)\big| \leq \frac{\max\left|\,f\,^{(n+1)}(z)\right|}{(n+1)!}\big|x^{(n+1)}\big|.$$
Since all derivatives of $\sin x$ are $\pm \cos x$ or $\pm\sin x$, whose magnitudes are bounded by $1$, we can state
$$ \big|R_n(x)\big| \leq \frac{1}{(n+1)!}\big|x^{(n+1)}\big|.$$
For any $x$, $\ds\lim_{n\to\infty} \frac{x^{n+1}}{(n+1)!} = 0$. Thus by the Squeeze Theorem, we conclude that $\ds \lim_{n\to\infty} R_n(x) = 0$ for all $x$, and hence
$$\sin x = \sum_{n=0}^\infty (-1)^{n}\frac{x^{2n+1}}{(2n+1)!}\quad \text{for all $x$}.$$
}
\exercise{$f(x) = \ln x$
}{Given a value $x$, the magnitude of the error term $R_n(x)$ is bounded by
$$ \big|R_n(x)\big| \leq \frac{\max\left|\,f\,^{(n+1)}(z)\right|}{(n+1)!}\big|(x-1)^{(n+1)}\big|,$$
where $z$ is between $1$ and $x$. 

Note that $\big|f\,^{(n+1)}(x)\big| = \frac{n!}{x^{n+1}}$. 

We consider the cases when $x>1$ and when $x<1$ separately.

If $x>1$, then $1<z<x$ and $f\,^{(n+1)}(z) =\frac{n!}{z^{n+1}}<n!$. Thus
$$ \big|R_n(x)\big| \leq \frac{n!}{(n+1)!}\big|(x-1)^{(n+1)}\big|= \frac{(x-1)^{n+1}}{n+1}.$$
For a fixed $x$,
$$\lim_{n\to\infty} \frac{(x-1)^{n+1}}{n+1}=0.$$


If $0<x<1$, then $x<z<1$ and $f\,^{(n+1)}(z) =\frac{n!}{z^{n+1}}<\frac{n!}{x^{n+1}}$. Thus
$$ \big|R_n(x)\big| \leq \frac{n!/x^{n+1}}{(n+1)!}\big|(x-1)^{(n+1)}\big| = \frac{x^{n+1}}{n+1}(1-x)^{n+1}.$$
Since $0<x<1$, $x^{n+1}<1$ and $(1-x)^{n+1}<1$. We can then extend the inequality from above to state
$$\big|R_n(x)\big| \leq \frac{x^{n+1}}{n+1}(1-x)^{n+1}<\frac1{n+1}.$$

As $n\to\infty$, $1/(n+1)\to0$. Thus by the Squeeze Theorem, we conclude that $\ds \lim_{n\to\infty} R_n(x) = 0$ for all $x$, and hence
$$\ln x = \sum_{n=1}^\infty (-1)^{n+1}\frac{(x-1)^{n}}{n}\quad \text{for all $0<x\leq 2$}.$$
}
\exercise{$f(x) = 1/(1-x)$ (show equality only on $(-1,0)$)
}{Given a value $x$, the magnitude of the error term $R_n(x)$ is bounded by
$$ \big|R_n(x)\big| \leq \frac{\max\left|\,f\,^{(n+1)}(z)\right|}{(n+1)!}\big|x^{(n+1)}\big|,$$
where $z$ is between $0$ and $x$. 

Note that $\big|f\,^{(n+1)}(x)\big| = \frac{(n+1)!}{(1-x)^{n+2}}$. 

%We consider the cases when $x>0$ and when $x<0$ separately.

If $0<x<1$, then $0<z<x$ and $f\,^{(n+1)}(z) =\frac{(n+1)!}{(1-z)^{n+2}}<\frac{(n+1)!}{(1-x)^{n+2}}$.
Thus
$$ \big|R_n(x)\big| \leq \frac{(n+1)!}{(1-x)^{n+2}}\frac{1}{(n+1)!}\big|x^{n+1}\big|= \frac{(x-1)^{n+1}}{n+1}.$$
For a fixed $x$,
$$\lim_{n\to\infty} \frac{(x-1)^{n+1}}{n+1}=0,$$
hence
$$\frac{1}{1-x} = \sum_{n=0}^\infty x^n \text{ on } (-1,0).$$
 
%If $-1<x<0$, then $x<z<0$ and $f\,^{(n+1)}(z) =\frac{(n+1)!}{(1-z)^{n+2}}<(n+1)!$. 
%Thus
%$$ \big|R_n(x)\big| \leq \frac{(n+1)!}{(n+1)!}\big|x^{n+1}\big|= \big|x^{n+1}\big|.$$
%For a fixed $x$,
%$$\lim_{n\to\infty} \big|x^{n+1}\big|=0 \text{ as } |x|<1.$$



%As $n\to\infty$, $1/(n+1)\to0$. Thus by the Squeeze Theorem, we conclude that $\ds \lim_{n\to\infty} R_n(x) = 0$ for all $x$, and hence
%$$\ln x = \sum_{n=1}^\infty (-1)^{n+1}\frac{(x-1)^{n}}{n}\quad \text{for all $0<x\leq 2$}.$$
}}