\exerciseset{In Exercises}{, an implicitly defined function of $x$, $y$ and $z$ is given along with a point $P$ that lies on the surface. Use the gradient $\nabla F$ to:
\begin{enumerate}
	\item [(a)] find the equation of the normal line to the surface at $P$, and
	\item	[(b)] find the equation of the plane tangent  to the surface at $P$.
\end{enumerate}
}{

\exercise{$\ds \frac{x^2}{8}+\frac{y^2}4+\frac{z^2}{16}=1$, at $P = (1,\sqrt{2},\sqrt{6})$
}{
$\nabla F = \la x/4, y/2, z/8\ra$; at $P$, $\nabla F = \la 1/4, \sqrt{2}/2, \sqrt{6}/8\ra$
\begin{enumerate}
	\item $\ell_{\vec n}(t) = \left\{\begin{array}{l} x= 1+ t/4 \\ y = \sqrt{2}+ \sqrt{2}t/2\\ z = \sqrt{6} + \sqrt{6}t/8 \end{array}\right.$
	\item		$\frac14(x-1) + \frac{\sqrt{2}}{2}(y-\sqrt{2}) + \frac{\sqrt{6}}8(z-\sqrt{6}) = 0$.
\end{enumerate}
}
\exercise{$\ds z^2-\frac{x^2}{4} - \frac{y^2}9=0$, at $P = (4,-3,\sqrt{5})$
}{
$\nabla F = \la -\frac x2, -\frac{2y}9,2z \ra$; at $P$, $\nabla F = \la -2, 2/3, 2\sqrt{5}\ra$
\begin{enumerate}
	\item $\ell_{\vec n}(t) = \left\{\begin{array}{l} x= 4-2t \\ y = -3+ 2t/3\\ z = \sqrt{5} + 2\sqrt{5}t \end{array}\right.$
	\item		$-2(x-4) + \frac23(y+3) + 2\sqrt{5}(z-\sqrt{5}) = 0$.
\end{enumerate}
}
\exercise{$\ds xy^2-xz^2=0$, at $P = (2,1,-1)$
}{
$\nabla F = \la y^2-z^2, 2xy, -2xz\ra$; at $P$, $\nabla F = \la 0, 4, 4\ra$
\begin{enumerate}
	\item $\ell_{\vec n}(t) = \left\{\begin{array}{l} x= 2 \\ y = 1+4t\\ z = -1+4t \end{array}\right.$
	\item		$4(y-1) + 4(z+1) = 0$.
\end{enumerate}
}
\exercise{$\ds \sin(xy)+\cos(yz)=0$, at $P = (2, \pi/12, 4)$
}{
$\nabla F = \la y\cos(xy), x\cos(xy)-z\sin(yz), -y\sin(yz)\ra$; at $P$, $\nabla F = \la \frac{\pi}{8\sqrt{3}}, -\sqrt{3},-\frac{\pi}{8\sqrt{3}}\ra$
\begin{enumerate}
	\item $\ell_{\vec n}(t) = \left\{\begin{array}{l} x= 2 +\frac{\pi}{8\sqrt{3}}t\\ y = \frac{\pi}{12}-\sqrt{3}t\\ z = 4-\frac{\pi}{8\sqrt{3}}t \end{array}\right.$
	\item		$\frac{\pi}{8\sqrt{3}}(x-2) -\sqrt{3}(y-\frac{\pi}{12}) -\frac{\pi}{8\sqrt{3}}(z-4) = 0$.
\end{enumerate}
}}